update gitignore and delete redundant files

coq/STLC.v
@@ -3,36 +3,44 @@ Inductive type : Type :=
   | N (*nat*)
   .
 
-Inductive num : Type :=
-  | zero
-  | succ (n : num).
-
 Inductive term : Type :=
   | boolean (b : bool)
   | if_then_else (t1 t2 t3 : term) (* if t1 then t2 else t3 *)
-  | number (n : num)
+  | zero
+  | succ (t: term) 
   | iszero (t : term)
   | pred (t : term).
 
+(* number value *)
+Inductive nvalue : term -> Prop :=
+  | NZero : nvalue zero
+  | NSucc : forall (t:term), nvalue t -> nvalue (succ t).
+
+Inductive value : term -> Prop :=
+  | BValue : forall (t : term) (b : bool), t = boolean b -> value t
+  | NValue : forall (t : term), nvalue t -> value t.
+
 Inductive evaluate : term -> term -> Prop :=
-  (** do not require [E_SUCC]: if t->t', then succ t -> succ t' here
-    since succ only accepts num value and no evaluation rule for
-    num exists. In other words, our language does not support
-    [succ (if_then_else true zero (succ zero))]*)
+  | E_SUCC :
+    forall (t1 t2 : term),
+    evaluate t1 t2 ->
+    evaluate (succ t1) (succ t2)
   | E_PREDZERO :
-    evaluate (pred (number zero)) (number zero)
+    evaluate (pred zero) zero
   | E_PREDSUCC :
-    forall (n : num),
-    evaluate (pred (number (succ n))) (number n)
+    forall (t : term),
+    nvalue t ->
+    evaluate (pred (succ t)) t
   | E_PRED :
     forall (t1 t2 : term),
     evaluate t1 t2 ->
     evaluate (pred t1) (pred t2)
   | E_ISZEROZERO :
-    evaluate (iszero (number zero)) (boolean true)
+    evaluate (iszero zero) (boolean true)
   | E_ISZEROSUCC :
-    forall (n:num),
-    evaluate (iszero (number (succ n))) (boolean false)
+    forall (t : term),
+    nvalue t ->
+    evaluate (iszero (succ t)) (boolean false)
   | E_ISZERO :
     forall (t1 t2 : term),
     evaluate t1 t2 ->
@@ -48,9 +56,8 @@ Inductive evaluate : term -> term -> Prop :=
     evaluate t1 t1' ->
     evaluate (if_then_else t1 t2 t3) (if_then_else t1' t2 t3).
 
-Inductive value : term -> Prop :=
-  | BValue : forall (t : term) (b : bool), t = boolean b -> value t
-  | NValue : forall (t : term) (n : num), t = number n -> value t.
+Notation "x \-> y" := (evaluate x y) (at level 50, left associativity).
+
 
 Inductive typeCheck : term -> type -> Prop :=
   | CheckTrue : typeCheck (boolean true) B
@@ -60,12 +67,11 @@ Inductive typeCheck : term -> type -> Prop :=
     typeCheck t2 T ->
     typeCheck t3 T ->
     typeCheck (if_then_else t1 t2 t3) T
-  | CheckZero : typeCheck (number zero) N
+  | CheckZero : typeCheck zero N
   | CheckSucc :
-    forall (t:term) (n:num),
+    forall (t:term),
     typeCheck t N ->
-    t = number n ->
-    typeCheck (number (succ n)) N
+    typeCheck (succ t) N
   | CheckPred :
     forall (t:term),
     typeCheck t N ->
@@ -75,38 +81,37 @@ Inductive typeCheck : term -> type -> Prop :=
     typeCheck t N ->
     typeCheck (iszero t) B.
 
+Notation "t :: T" := (typeCheck t T).
+
 (* A trick here *)
 Lemma typeCheck_number_is_not_B:
-forall (n : num), typeCheck (number n) B -> False.
+forall t, nvalue t -> t :: B -> False.
 Proof.
   intros. 
-  remember (number n) as t.
-  (*I need to remember B. Otherwise B will disappear*)
-  remember B as type_.
-  induction H; try discriminate. 
+  induction H; inversion H0. 
 Qed.
 
 (** [Canonical Form (Page 127) (1)] If [v] is a value of type [Bool],
 then [v] is either [true] or [false]*)
 Lemma boolvalue_only_contains_true_or_false :
-forall (t:term), value t -> typeCheck t B -> t = boolean true \/ t = boolean false.
+forall (t:term), value t -> t :: B -> t = boolean true \/ t = boolean false.
 Proof.
-  intros. induction t eqn:E.
-  - destruct b. left; reflexivity. right; reflexivity.
-  - rewrite <- E in H. destruct H eqn:E'; rewrite e in E; discriminate.
-  - rewrite <- E in H0. rewrite E in H0. apply typeCheck_number_is_not_B in H0.
-    contradiction.
-  - destruct H eqn:E'. destruct b eqn:E''. left. apply e. right. apply e. 
-    rewrite e in H0. apply typeCheck_number_is_not_B in H0. contradiction.
-  - remember (pred t0) as predn.
-    destruct H eqn:E'. destruct b; rewrite e. left; reflexivity. right; reflexivity.
-    rewrite e in Heqpredn. discriminate.
+  intros. remember t as t'. remember B as T. induction H0.
+  - left. reflexivity.
+  - right. reflexivity.
+  - inversion H. discriminate. inversion H0.
+  - discriminate.
+  - discriminate.
+  - discriminate.
+  - inversion H.
+    + discriminate.
+    + inversion H1. 
 Qed.
 
-(** [Canonical Form (Page 128) (2)] If [v] is a value of type [Nat],
+(* (** [Canonical Form (Page 128) (2)] If [v] is a value of type [Nat],
 then [v] is a [number]*)
-Lemma numvalue_only_contains_zero_of_succ :
-forall (t:term),  value t -> typeCheck t N -> exists (n:num), t = number n.
+Lemma numvalue_only_contains_zero_or_succ :
+forall (t:term), nvalue t -> t = zero \/ exists (t' : term), nvalue t' -> 
 Proof.
   intros. remember N as type_. induction H0; try discriminate.
   - remember (if_then_else t1 t2 t3) as ifH. destruct H; rewrite HeqifH in H;
@@ -117,89 +122,120 @@ Proof.
     destruct H eqn:E.
     + rewrite e in Heqpredn; discriminate.
     + rewrite e. exists n; reflexivity. 
-Qed.
+Qed. *)
+
 
 (* [exists (tp : type), typeCheck t tp] means term [t] is well-typed *)
-Theorem Progress : forall (t:term), (exists (tp : type), typeCheck t tp) -> 
-  value t \/ (exists (t':term), evaluate t t').
+Theorem Progress : forall (t:term), (exists (tp : type), t :: tp) -> 
+  value t \/ (exists (t':term), t \-> t').
 Proof. 
-  intros. destruct H. induction H.
-  - left. apply BValue with (b:=true); reflexivity.
-  - left. apply BValue with (b:=false); reflexivity.
-  - right. destruct IHtypeCheck1.
-    + apply boolvalue_only_contains_true_or_false in H2.
-      destruct H2. 
-      -- exists t2. rewrite H2. apply E_IFTRUE.
-      -- exists t3. rewrite H2. apply E_IFFALSE.
-      -- apply H.
-    + destruct H2. apply E_IF with (t2:=t2) (t3:=t3) in H2.
-      exists (if_then_else x t2 t3). apply H2.
-  - left. apply NValue with (n:=zero). reflexivity.
-  - left. apply NValue with (n:=succ n). reflexivity.
+  intros. destruct H. 
+  induction H.
+  - left. apply BValue with (b:=true). reflexivity.
+  - left. apply BValue with (b:=false). reflexivity.
+  - right.  
+    destruct IHtypeCheck1.
+    + inversion H2.
+      -- destruct b; rewrite H3.
+         ++ exists t2. apply E_IFTRUE.
+         ++ exists t3. apply E_IFFALSE.
+      -- inversion H3; inversion H.
+         ++ rewrite <- H5 in H6; discriminate.
+         ++ rewrite <- H5 in H6; discriminate.
+         ++ rewrite <- H5 in H9; discriminate.
+         ++ rewrite <- H5 in H7; discriminate.
+         ++ rewrite <- H6 in H7; discriminate.
+         ++ rewrite <- H6 in H7; discriminate.
+         ++ rewrite <- H6 in H10; discriminate.
+         ++ rewrite <- H6 in H8; discriminate.
+    + destruct H2.
+      exists (if_then_else x t2 t3).
+      apply E_IF.
+      apply H2.
+  - left. apply NValue. apply NZero.
+  - destruct IHtypeCheck.
+    + left. apply NValue. inversion H0.
+      -- rewrite H1 in H. inversion H.
+      -- apply NSucc. apply H1.
+    + destruct H0.
+      right. exists (succ x).
+      apply E_SUCC. apply H0.
   - right.
     destruct IHtypeCheck.
-    + apply numvalue_only_contains_zero_of_succ in H.
-      -- destruct H. destruct x eqn:Ex.
-         ++ rewrite H. exists (number zero).
-            apply E_PREDZERO.
-         ++ rewrite H. exists (number n).
-            apply E_PREDSUCC.
-      -- apply H0.
-    + destruct H0. exists (pred x).
-      apply E_PRED. apply H0.
-  - destruct IHtypeCheck.
+    + inversion H0.
+      -- rewrite H1 in H. inversion H.
+      -- destruct H1.
+         ++ exists zero. apply E_PREDZERO.
+         ++ exists t. apply E_PREDSUCC. apply H1.
     + destruct H0.
-      -- apply numvalue_only_contains_zero_of_succ in H.
-         destruct H. rewrite H in H0. discriminate.
-         rewrite H0. apply BValue with (b:=b). reflexivity.
-      -- destruct n eqn:En.
-         ++ right. rewrite H0. exists (boolean true).
-            apply E_ISZEROZERO.
-         ++ right. rewrite H0. exists (boolean false).
-            apply E_ISZEROSUCC.
-    + destruct H0. right. exists (iszero x). apply E_ISZERO.
+      exists (pred x).
+      apply E_PRED.
       apply H0.
-Qed.
+  - right. destruct IHtypeCheck.
+    + inversion H0.
+      -- rewrite H1 in H. inversion H.
+      -- destruct H1.
+         ++ exists (boolean true). apply E_ISZEROZERO.
+         ++ exists (boolean false). apply E_ISZEROSUCC. apply H1.
+    + destruct H0.
+      exists (iszero x).
+      apply E_ISZERO.
+      apply H0.
+Qed. 
 
 Axiom pred_succ_is_itself:
-forall (n:num), pred (number (succ n)) = number n.
+forall (t:term), pred (succ t) = t.
+
+Lemma succ_t_is_of_N_then_t_is_also_of_N :
+forall (t:term), succ t :: N -> t :: N.
+Proof.
+  intros.
+  inversion H.
+  apply H1.
+Qed.
 
 (** If [t] : [T] and [t] -> [t'], then [t'] : [T]*)
 Theorem Preservation :
-forall (t t':term) (T:type), typeCheck t T -> evaluate t t' -> typeCheck t' T.
+forall (t t':term) (T:type), t :: T -> (t \-> t') -> t' :: T.
 Proof. (* induction on type system , could also do induction on evaluation*)
-  intros. generalize dependent t'. induction H.
-  - remember (boolean true) as btrue. intros.
-    induction H0; try discriminate.
-  - remember (boolean false) as bfalse. intros.
-    induction H0; try discriminate.
-  - remember (if_then_else t1 t2 t3) as ifH. 
-    intros. destruct H2; try discriminate.
-    + injection HeqifH; intros. rewrite H3. apply H0.
-    + injection HeqifH; intros. rewrite H2. apply H1.
-    + injection HeqifH; intros. rewrite H3. rewrite H4. 
-      clear HeqifH. clear H3. clear H4. rewrite H5 in H2. clear H5.
+  intros.
+  generalize dependent t'.
+   induction H; intros.
+  - inversion H0. (* cannot evaluate (boolean true)*)
+  - inversion H0. (* cannot evaluate (boolean false)*)
+  - remember B as B'. destruct H.
+    + inversion H2.
+      -- rewrite <- H5. apply H0.
+      -- inversion H6.
+    + inversion H2.
+      -- rewrite <- H5. apply H1.
+      -- inversion H6.
+    + rewrite HeqB' in H3;
+      rewrite HeqB' in H4;
+      rewrite HeqB' in IHtypeCheck1.
+      clear HeqB'.
+      inversion H2.
       apply CheckIf.
-      apply IHtypeCheck1 in H2. apply H2.
-      apply H0.
-      apply H1.
-  - intros. remember (number zero) as Hzero. destruct H0; try discriminate.
-  - intros. remember (number (succ n)) as Hsucc.
-    destruct H1; try discriminate. 
-  - intros. remember (pred t) as Hpredt.
-    destruct H0; try discriminate.
+      -- apply IHtypeCheck1 in H9. apply H9. (* auto *)
+      -- apply H0.
+      -- apply H1.
+    + discriminate.
+    + discriminate.
+    + discriminate.
+    + inversion H2. apply CheckIf.
+      -- auto.
+      -- apply H0.
+      -- apply H1.
+  - inversion H0.
+  - inversion H0; clear H1.
+    apply IHtypeCheck in H2. apply CheckSucc. apply H2.
+  - inversion H0.
     + apply CheckZero.
-    + injection HeqHpredt; intros; clear HeqHpredt; rewrite <- H0 in IHtypeCheck;
-      rewrite <- H0 in H. rewrite <- pred_succ_is_itself.
-      apply CheckPred. apply H.
-    + injection HeqHpredt; intros. rewrite H1 in H0. clear H1. clear HeqHpredt.
-      apply IHtypeCheck in H0. apply CheckPred. apply H0.
-  - intros. remember (iszero t) as Hiszero.
-    destruct H0; try discriminate.
+    + rewrite <- H1 in H; rewrite <- H3.
+      apply succ_t_is_of_N_then_t_is_also_of_N in H. apply H.
+    + apply IHtypeCheck in H2. apply CheckPred. apply H2.
+  - inversion H0.
     + apply CheckTrue.
     + apply CheckFalse.
-    + injection HeqHiszero; intros. rewrite H1 in H0. clear HeqHiszero. clear H1.
-      apply IHtypeCheck in H0. apply CheckIszero. apply H0.
+    + apply IHtypeCheck in H2. apply CheckIszero. apply H2.             
 Qed.
-
-
